Chapter 6 Homework Done

lean/LoVe/LoVe06_InductivePredicates_HomeworkSheet.lean
@@ -79,6 +79,9 @@ would use replace `(step)` with the following right-leaning rule:
 Define a predicate `TCV2` that embodies this alternative definition. -/
 
 -- enter your definition here
+inductive TCV2 {α : Type} (R : α → α → Prop) : α → α → Prop
+  | base (a b : α) : R a b → TCV2 R a b
+  | step (a b c : α) : TCV2 R a b → R b c → TCV2 R a c
 
 /- 2.2 (2 points). Yet another definition of the transitive closure `R⁺` would
 use the following symmetric rule instead of `(step)` or `(pets)`:
@@ -88,18 +91,37 @@ use the following symmetric rule instead of `(step)` or `(pets)`:
 Define a predicate `TCV3` that embodies this alternative definition. -/
 
 -- enter your definition here
+inductive TCV3 {α : Type} (R : α → α → Prop) : α → α → Prop
+  | base (a b : α) : R a b → TCV3 R a b
+  | step (a b c : α) : TCV3 R a b → TCV3 R b c → TCV3 R a c
 
 /- 2.3 (1 point). Prove that `(step)` also holds as a theorem about `TCV3`. -/
 
 theorem TCV3_step {α : Type} (R : α → α → Prop) (a b c : α) (rab : R a b)
     (tbc : TCV3 R b c) :
   TCV3 R a c :=
-  sorry
-
+  by
+    apply TCV3.step a b c
+    {
+      apply TCV3.base
+      exact rab
+    }
+    { exact tbc }
 /- 2.4 (1 point). Prove the following theorem by rule induction: -/
 
 theorem TCV1_pets {α : Type} (R : α → α → Prop) (c : α) :
   ∀a b, TCV1 R a b → R b c → TCV1 R a c :=
-  sorry
+  by
+    intro a b
+    intro trab rbc
+    induction trab with
+    | base a' b' rab => {
+      exact TCV1.step a' b' c (rab) (TCV1.base b' c (rbc))
+    }
+    | step a' b' c' rab trbc ih => {
+      apply TCV1.step a' b' c
+      { exact rab }
+      { exact (ih rbc) }
+    }
 
 end LoVe
